1. Let $R$ be a commutative ring. Suppose $f_0 \in R, f_1 \in R[x_1], f_2 \in R[x_1, x_2], \ldots, f_n \in R[x_1, \ldots, x_n]$ be arbitrary polynomials of $0,1, \ldots n$ variables. Then the quotient $R[x_1, \ldots, x_{n+1}] /(x_1-f_0, x_2-f_1(x_1), \ldots, x_{n+1}-f_n(x_1, \ldots, x_n))$ is isomorphic to $R$.
    
    **Proof**
    
    The evaluation homomorphism $\phi: P \to R$ is defined by sending each indeterminate $x_i$ (for $i = 1, \dots, n+1$) to the corresponding element $s_{i-1} \in R$, where $s_0 = f_0$ and $s_k = f_k(s_0, s_1, \dots, s_{k-1})$ for $k = 1, \dots, n$.
    
    Explicitly, for any polynomial $p \in P$, $\phi(p)$ is the element in $R$ obtained by substituting $x_i \mapsto s_{i-1}$ for each $i$ and evaluating the resulting expression in $R$.
    
    Since $R$ is commutative, this substitution preserves addition and multiplication, ensuring $\phi$ is a ring homomorphism.
    
    - Surjectivity of $\phi$
    
        Since $\phi$ fixes any constant polynomial $r \in R \subset P$, the image of $\phi$ contains all of $R$. As the codomain of $\phi$ is also $R$, the image must be exactly $R$, which means $\phi$ is surjective.
    
    - $\ker(ϕ) ⊇ I$
    
        By the definition of the evaluation homomorphism $\phi: P \to R$, $\phi(x_i - f_{i-1}(x_1, \dots, x_{i-1})) = s_{i-1} - f_{i-1}(s_0, \dots, s_{i-2}) = s_{i-1} - s_{i-1} = 0$, where the last equality holds by the recursive definition of $(s_k)$.
    
        Thus, since $\phi$ is a ring homomorphism that maps every generator of $I$ to zero, it maps the entire ideal to zero, meaning $I \subseteq \ker(\phi)$.
    
    - $\ker(ϕ) ⊆ I$
    
        To prove that $\ker(\phi) \subseteq I$, proceed by induction on the number of recursive relations (or equivalently, on the index $n$, where the polynomial ring has $n+1$ indeterminates).
        
        For the base case with no recursive relations beyond a single variable ($n = 0$), consider $P = R[x_1]$ and $I = (x_1 - f_0)$ with $f_0 \in R$ constant and $\phi(x_1) = f_0 = s_0$. Any polynomial $g \in P$ can be written uniquely as $g = q(x_1)(x_1 - f_0) + r$ where $r \in R$ is the remainder (constant term after division by the monic linear polynomial $x_1 - f_0$). Applying $\phi$ gives $\phi(g) = \phi(r) = r$, since $\phi(x_1 - f_0) = 0$. If $g \in \ker(\phi)$, then $r = 0$, so $g = q(x_1)(x_1 - f_0) \in I$. Thus $\ker(\phi) \subseteq I$.
        
        Now assume the result holds for fewer than $n+1$ indeterminates (induction hypothesis). For the general case, let $Q = R[x_1, \dots, x_n]$ so that $P = Q[x_{n+1}]$, and let $I'$ be the ideal in $Q$ generated by the first $n$ relations: $I' = (x_1 - f_0, x_2 - f_1(x_1), \dots, x_n - f_{n-1}(x_1, \dots, x_{n-1}))$. Then $I = I' \cdot P + (x_{n+1} - f_n(x_1, \dots, x_n))$, where $f_n \in Q$.
        
        Take any $g \in \ker(\phi)$, so $\phi(g) = g(s_0, \dots, s_n) = 0$. Since $x_{n+1} - f_n$ is monic in $x_{n+1}$, the division algorithm in $Q[x_{n+1}]$ yields unique $q \in P$ and $r \in Q$ such that
        
        $g = q \cdot (x_{n+1} - f_n) + r.$
        
        Applying $\phi$ gives
        
        $\phi(g) = \phi(q) \cdot \phi(x_{n+1} - f_n) + \phi(r) = 0 + \phi(r) = r(s_0, \dots, s_{n-1}) = 0,$
        
        since $\phi(x_{n+1} - f_n) = s_n - f_n(s_0, \dots, s_{n-1}) = 0$ by the recursive definition of the $s_i$. Thus $r$ lies in the kernel of the evaluation homomorphism from $Q$ to $R$ sending $x_i \mapsto s_{i-1}$ for $i = 1, \dots, n$. By the induction hypothesis, $r \in I'$.
        
        It follows that
        
        $g = q \cdot (x_{n+1} - f_n) + r \in (x_{n+1} - f_n) \cdot P + I' \cdot P \subseteq I.$
        
        Hence $g \in I$, completing the induction.
        
    - Conclusion
    
        By the First Isomorphism Theorem for rings, since $\mathrm{im}(\phi) = R$ and $\ker(\phi) = I$, it follows that $P / I \cong R$. This completes the proof.
2. Let $\varphi: R \rightarrow R'$ be a map of rings, $\mathfrak{a}$ an ideal of $R$, and $\mathfrak{b}$ an ideal of $R'$. Prove the following statements:
    1. Then $\mathfrak{a}^{ec} \supset \mathfrak{a}$ and $\mathfrak{b}^{ce} \subset \mathfrak{b}$.
    2. Then $\mathfrak{a}^{ece}=\mathfrak{a}^e$ and $\mathfrak{b}^{cec}=\mathfrak{b}^c$.
    3. If $\mathfrak{b}$ is an extension, then $\mathfrak{b}^c$ is the largest ideal of $R$ with extension $\mathfrak{b}$.
    4. If two extensions have the same contraction, then they are equal.
    
    **Proof**
    1. For any ideal $\mathfrak{a} \subseteq R$, we have $\mathfrak{a} \subseteq \varphi^{-1}(\varphi(\mathfrak{a}))$. Since $\mathfrak{a}^e$ is the ideal generated by $\varphi(\mathfrak{a})$, we have $\varphi(\mathfrak{a}) \subseteq \mathfrak{a}^e$. Applying $\varphi^{-1}$ to this inclusion gives $\varphi^{-1}(\varphi(\mathfrak{a})) \subseteq \varphi^{-1}(\mathfrak{a}^e) = \mathfrak{a}^{ec}$. Combining these, we get $\mathfrak{a} \subseteq \mathfrak{a}^{ec}$.

       For any ideal $\mathfrak{b} \subseteq R'$, we have $\varphi(\varphi^{-1}(\mathfrak{b})) \subseteq \mathfrak{b}$. By definition, $\mathfrak{b}^c = \varphi^{-1}(\mathfrak{b})$, so $\varphi(\mathfrak{b}^c) \subseteq \mathfrak{b}$. Since $\mathfrak{b}^{ce}$ is the ideal generated by $\varphi(\mathfrak{b}^c)$ and $\mathfrak{b}$ is an ideal, it follows that $\mathfrak{b}^{ce} \subseteq \mathfrak{b}$.
    2. For $\mathfrak{a}^{ece}=\mathfrak{a}^e$:
       From (1), $\mathfrak{a} \subseteq \mathfrak{a}^{ec}$. Applying extension gives $\mathfrak{a}^e \subseteq (\mathfrak{a}^{ec})^e = \mathfrak{a}^{ece}$.
       Also from (1), $\mathfrak{b}^{ce} \subseteq \mathfrak{b}$ for any ideal $\mathfrak{b} \subseteq R'$. Let $\mathfrak{b} = \mathfrak{a}^e$, then $(\mathfrak{a}^e)^{ce} \subseteq \mathfrak{a}^e$, so $\mathfrak{a}^{ece} \subseteq \mathfrak{a}^e$.
       Thus, $\mathfrak{a}^{ece} = \mathfrak{a}^e$.

       For $\mathfrak{b}^{cec}=\mathfrak{b}^c$:
       From (1), $\mathfrak{b}^{ce} \subseteq \mathfrak{b}$. Applying contraction gives $(\mathfrak{b}^{ce})^c \subseteq \mathfrak{b}^c$, so $\mathfrak{b}^{cec} \subseteq \mathfrak{b}^c$.
       Also from (1), $\mathfrak{a} \subseteq \mathfrak{a}^{ec}$ for any ideal $\mathfrak{a} \subseteq R$. Let $\mathfrak{a} = \mathfrak{b}^c$, then $\mathfrak{b}^c \subseteq (\mathfrak{b}^c)^{ec} = \mathfrak{b}^{cec}$.
       Thus, $\mathfrak{b}^{cec} = \mathfrak{b}^c$.
    3. To show $\mathfrak{b}^c$ is the largest ideal with extension $\mathfrak{b}$:
       - $(\mathfrak{b}^c)^e = \mathfrak{b}^{ce} = \mathfrak{b}$ since $\mathfrak{b}$ is an extension (by (2)).
       - If $\mathfrak{a}^e = \mathfrak{b}$, then $\mathfrak{a} \subseteq \mathfrak{a}^{ec} = \mathfrak{b}^c$ by (1).
    4. Let $\mathfrak{b}_1, \mathfrak{b}_2$ be extensions with $\mathfrak{b}_1^c = \mathfrak{b}_2^c$. Since any extension $\mathfrak{b}$ satisfies $\mathfrak{b} = \mathfrak{b}^{ce} = (\mathfrak{b}^c)^e$ by (2), we have $\mathfrak{b}_1 = (\mathfrak{b}_1^c)^e = (\mathfrak{b}_2^c)^e = \mathfrak{b}_2$.
3. (Chinese Remainder Theorem) Let $R$ be a ring.
    1. Let $\mathfrak{a}$ and $\mathfrak{b}$ be comaximal ideals; that is, $\mathfrak{a}+\mathfrak{b}=R$. Show
        1. $\mathfrak{a b}=\mathfrak{a} \cap \mathfrak{b} \quad$ and
        2. $R / \mathfrak{a b}=(R / \mathfrak{a}) \times(R / \mathfrak{b})$.
    2. Let $\mathfrak{a}$ be comaximal to both $\mathfrak{b}$ and $\mathfrak{b}'$. Show $\mathfrak{a}$ is also comaximal to $\mathfrak{b} \mathfrak{b}'$.
    3. Given $m, n \geq 1$, show $\mathfrak{a}$ and $\mathfrak{b}$ are comaximal if and only if $\mathfrak{a}^m$ and $\mathfrak{b}^n$ are.
    4. Let $\mathfrak{a}_1, \ldots, \mathfrak{a}_n$ be pairwise comaximal.
        1. $\mathfrak{a}_1$ and $\mathfrak{a}_2 \cdots \mathfrak{a}_n$ are comaximal;
        2. $\mathfrak{a}_1 \cap \cdots \cap \mathfrak{a}_n=\mathfrak{a}_1 \cdots \mathfrak{a}_n$;
        3. $R /\left(\mathfrak{a}_1 \cdots \mathfrak{a}_n\right) \xrightarrow{\sim} \prod\left(R / \mathfrak{a}_i\right)$.
    5. Find an example where $\mathfrak{a}$ and $\mathfrak{b}$ satisfy (1)(a), but aren't comaximal.
    
    **Proof**
    1. Let $\mathfrak{a}+\mathfrak{b}=R$. Then $1=a+b$ for some $a\in\mathfrak{a},b\in\mathfrak{b}$.
        1. $\mathfrak{a b}\subseteq\mathfrak{a}\cap\mathfrak{b}$ always holds. For the opposite inclusion, let $x\in\mathfrak{a}\cap\mathfrak{b}$, then $x=xa+xb\in\mathfrak{a b}$ because both $xa,xb\in\mathfrak{a b}$.
        2. The homomorphism $R\to (R / \mathfrak{a}) \times(R / \mathfrak{b})$ is surjective (since $\mathfrak{a}, \mathfrak{b}$ are comaximal) and has kernel $\mathfrak{a}\cap\mathfrak{b}=\mathfrak{a b}$. By the First Isomorphism Theorem, $R/\mathfrak{ab}\cong R/\mathfrak{a}\times R/\mathfrak{b}$.
    2. If $\mathfrak{a}$ is comaximal to both $\mathfrak{b}$ and $\mathfrak{b}'$, then $R=RR=(\mathfrak{a}+\mathfrak{b})(\mathfrak{a}+\mathfrak{b}') \subseteq \mathfrak{a}+\mathfrak{b} \mathfrak{b}' \subseteq R$, so $\mathfrak{a}+\mathfrak{b}\mathfrak{b}'=R.
    3. ($\Rightarrow$) If $\mathfrak{a}+\mathfrak{b}=R$, then $R = (\mathfrak{a}+\mathfrak{b})^{m+n-1} \subseteq \mathfrak{a}^m+\mathfrak{b}^n$, so $\mathfrak{a}^m+\mathfrak{b}^n=R$.
        
        ($\Leftarrow$) If $\mathfrak{a}^m+\mathfrak{b}^n=R$, then $R = \mathfrak{a}^m+\mathfrak{b}^n \subseteq \mathfrak{a}+\mathfrak{b}$, so $\mathfrak{a}+\mathfrak{b}=R$.
    4. Let $\mathfrak{a}_1, \ldots, \mathfrak{a}_n$ be pairwise comaximal. Show:
        1. Use 2. inductively.
        2. Use 1(a) inductively.
        3. Use 1(b) inductively.
    5. $R=\mathbb{Z},\mathfrak{a}=(0),\mathfrak{b}=(2)$. Then $\mathfrak{a b}=(0)(2)=(0)$ and $\mathfrak{a} \cap \mathfrak{b}=(0) \cap (2)=(0)$, so $\mathfrak{a b}=\mathfrak{a} \cap \mathfrak{b}$. However, $\mathfrak{a}+\mathfrak{b}=(0)+(2)=(2)\neq\mathbb{Z}$, so they are not comaximal.

4. Let $R:=R' \times R''$ be a product of rings, $\mathfrak{a} \subset R$ an ideal.
   1. Show $\mathfrak{a}=\mathfrak{a}' \times \mathfrak{a}''$ with $\mathfrak{a}' \subset R'$ and $\mathfrak{a}'' \subset R''$ ideals.
   2. Show $R / \mathfrak{a} \cong \left(R' / \mathfrak{a}'\right) \times\left(R'' / \mathfrak{a}''\right)$.

    Proof

    1. Define $`\mathfrak{a}' = \{ r' \in R' \mid (r', 0) \in \mathfrak{a} \}`$ and $`\mathfrak{a}'' = \{ r'' \in R'' \mid (0, r'') \in \mathfrak{a} \}`$. Note that $\mathfrak{a}'$ is the image of $\mathfrak{a}$ under the projection map $R \to R'$, and is therefore an ideal in $R'$; similarly for $\mathfrak{a}''$.

        Then $\mathfrak{a} = \mathfrak{a}' \times \mathfrak{a}''$:
       
        $\mathfrak{a}' \times \mathfrak{a}'' \subseteq \mathfrak{a}$: If $a' \in \mathfrak{a}'$ and $a'' \in \mathfrak{a}''$, then $(a', 0) \in \mathfrak{a}$ and $(0, a'') \in \mathfrak{a}$, so $(a', a'') = (a', 0) + (0, a'') \in \mathfrak{a}$ as ideals are closed under addition.

        $\mathfrak{a} \subseteq \mathfrak{a}' \times \mathfrak{a}''$: If $(r', r'') \in \mathfrak{a}$, then $(r', 0) = (r', r'') \cdot (1', 0) \in \mathfrak{a}$ (since $\mathfrak{a}$ is an ideal) and $(0, r'') = (r', r'') \cdot (0, 1'') \in \mathfrak{a}$, so $r' \in \mathfrak{a}'$ and $r'' \in \mathfrak{a}''$.
    2. To show $R / \mathfrak{a} \cong (R' / \mathfrak{a}') \times (R'' / \mathfrak{a}'')$, we use the result from part 1 that $\mathfrak{a} = \mathfrak{a}' \times \mathfrak{a}''$. We need to show $(R' \times R'') / (\mathfrak{a}' \times \mathfrak{a}'') \cong (R' / \mathfrak{a}') \times (R'' / \mathfrak{a}'')$.

       Consider the natural projection map $\phi: R' \times R'' \to (R' / \mathfrak{a}') \times (R'' / \mathfrak{a}'')$ given by $\phi((r', r'')) = (r' + \mathfrak{a}', r'' + \mathfrak{a}'')$. This is a surjective ring homomorphism with kernel $\mathfrak{a}' \times \mathfrak{a}''$. By the First Isomorphism Theorem for rings, the desired isomorphism holds.

5. Let $\mathfrak{a}$ and $\mathfrak{b}$ be ideals, and $\mathfrak{p}$ a prime ideal. Prove that these conditions are equivalent: (1) $\mathfrak{a} \subset \mathfrak{p}$ or $\mathfrak{b} \subset \mathfrak{p}$; and (2) $\mathfrak{a} \cap \mathfrak{b} \subset \mathfrak{p} ;$ and (3) $\mathfrak{a b} \subset \mathfrak{p}$.

   (1) ⇒ (3): If $\mathfrak{a} \subseteq \mathfrak{p}$, then $\mathfrak{a}\mathfrak{b} \subseteq \mathfrak{p}\mathfrak{b} \subseteq \mathfrak{p}$ (since $\mathfrak{p}$ is an ideal). Similarly if $\mathfrak{b} \subseteq \mathfrak{p}$.

   (3) ⇒ (2): If $\mathfrak{a}\mathfrak{b} \subseteq \mathfrak{p}$ and $x \in \mathfrak{a} \cap \mathfrak{b}$, then $x^2 = x \cdot x \in \mathfrak{a}\mathfrak{b} \subseteq \mathfrak{p}$. Since $\mathfrak{p}$ is prime, $x^2 \in \mathfrak{p}$ implies $x \in \mathfrak{p}$. Thus $\mathfrak{a} \cap \mathfrak{b} \subseteq \mathfrak{p}$.

   (2) ⇒ (1): Suppose neither containment holds. Let $a \in \mathfrak{a} \setminus \mathfrak{p}$ and $b \in \mathfrak{b} \setminus \mathfrak{p}$. Then $ab \in \mathfrak{a}$ (since $\mathfrak{a}$ is an ideal) and $ab \in \mathfrak{b}$ (since $\mathfrak{b}$ is an ideal), so $ab \in \mathfrak{a} \cap \mathfrak{b} \subseteq \mathfrak{p}$. Since $\mathfrak{p}$ is prime, $ab \in \mathfrak{p}$ implies $a \in \mathfrak{p}$ or $b \in \mathfrak{p}$, a contradiction.

6. Let $R$ be a ring, $\mathfrak{p}$ a prime ideal, and $\mathfrak{m}_1, \ldots, \mathfrak{m}_n$ maximal ideals. Assume $\mathfrak{m}_1 \cdots \mathfrak{m}_n=0$. Show $\mathfrak{p}=\mathfrak{m}_i$ for some $i$.

   **Proof**

   We are given that $\mathfrak{m}_1 \cdots \mathfrak{m}_n = (0)$. Since $\mathfrak{p}$ is a prime ideal, it contains $(0)$, so $\mathfrak{m}_1 \cdots \mathfrak{m}_n \subseteq \mathfrak{p}$. By induction on $n$ using Q5 (3) ⇒ (1), this implies $\mathfrak{m}_i \subseteq \mathfrak{p}$ for some index $i$.

   Since $\mathfrak{m}_i$ is a maximal ideal and $\mathfrak{p}$ is a proper ideal, the inclusion $\mathfrak{m}_i \subseteq \mathfrak{p}$ forces equality. Thus, $\mathfrak{p} = \mathfrak{m}_i$.
