Problems based on Tuesday 1/20 lecture:
1. Two Riemannian metrics $g$ and $h$ on the same manifold $M$ are said to be conformal if there exists a positive smooth function $f(x)$ such that
  $g=f \cdot h .$

    Show that angles between tangent vectors are the same with respect to $g$ and $h$.
    
    The cosine of the angle between two tangent vectors $X_1, X_2 \in T_p M$ with respect to $g$ is given by

   $\cos \theta_g = \frac{g(X_1, X_2)}{\sqrt{g(X_1, X_1) g(X_2, X_2)}}.$

    If $g = f h$ with $f > 0$, then

    $\cos \theta_g = \frac{f h(X_1, X_2)}{\sqrt{f h(X_1, X_1) \cdot f h(X_2, X_2)}} = \frac{f h(X_1, X_2)}{f \sqrt{h(X_1, X_1) h(X_2, X_2)}} = \frac{h(X_1, X_2)}{\sqrt{h(X_1, X_1) h(X_2, X_2)}} = \cos \theta_h.$

    Thus, the scaling factor $f$ cancels out, ensuring that angles are identical for conformally equivalent metrics.

2. Show that the round metric on $S^n$ is given in stereographic coordinates by

   $$g_{i j}=\frac{4 \delta_{i j}}{\left(1+|x|^2\right)^2} .$$

    For the unit n-sphere $S^n$ embedded in $\mathbb{R}^{n+1}$ with the standard Euclidean metric, the inverse stereographic projection $\Phi: \mathbb{R}^n \to S^n \subset \mathbb{R}^{n+1}$ from the North Pole $(0,\dots,0,1)$ is given by:

    $$u^i = \frac{2x^i}{1+|x|^2} \quad \text{for } i=1,\dots,n,$$

    $$u^{n+1} = \frac{|x|^2 - 1}{|x|^2 + 1} = 1 - \frac{2}{1+|x|^2},$$

    where $|x|^2 = \sum_{k=1}^n (x^k)^2$.

    When we use stereographic coordinates $x^{i}$, we are defining an embedding map $\Phi :\mathbb{R}^{n}\rightarrow \mathbb{R}^{n+1}$ where each ambient coordinate $u^{k}$ is a function of the local coordinates, $u^{k}=u^{k}(x^{1},\dots ,x^{n})$. The induced metric is found by pulling back the Euclidean metric from $\mathbb{R}^{n+1}$. The Euclidean line element is $ds^{2} = \sum_{k=1}^{n+1} (du^k)^2$. The differential of each ambient coordinate is:

   $`du^{k}=\sum _{i=1}^{n}\frac{\partial u^{k}}{\partial x^{i}}dx^{i}`$

   Substituting this into the line element:
   
    $`ds^{2}=\sum _{k=1}^{n+1}\left(\sum _{i=1}^{n}\frac{\partial u^{k}}{\partial x^{i}}dx^{i}\right)\left(\sum _{j=1}^{n}\frac{\partial u^{k}}{\partial x^{j}}dx^{j}\right)`$

   Rearranging the sums to group the $dx^{i}dx^{j}$ terms gives the line element in local coordinates:
   
    $`ds^{2}=\sum _{i,j=1}^{n}\left(\sum _{k=1}^{n+1}\frac{\partial u^{k}}{\partial x^{i}}\frac{\partial u^{k}}{\partial x^{j}}\right)dx^{i}dx^{j}`$

   By definition, the components of the metric tensor $g_{ij}$ are the coefficients of $dx^{i}dx^{j}$, so:

   $`g_{ij}=\sum _{k=1}^{n+1}\frac{\partial u^{k}}{\partial x^{i}}\frac{\partial u^{k}}{\partial x^{j}}`$

   Pullback the round metric on $S^n$ to stereographic coordinates on $\mathbb{R}^n$ by computing the partial derivatives of the embedding $\Phi$. Let $D = 1 + |x|^2$. Then:

    $$\frac{\partial u^k}{\partial x^i} = \frac{2 \delta_{ki} D - 4 x^k x^i}{D^2} \quad \text{for } k \leq n,$$

    $$\frac{\partial u^{n+1}}{\partial x^i} = \frac{4 x^i}{D^2}.$$

    The metric components are $g_{ij} = \sum_{k=1}^{n+1} \frac{\partial u^k}{\partial x^i} \frac{\partial u^k}{\partial x^j}$, which expands to:

    $$g_{ij} = \sum_{k=1}^{n} \left( \frac{2 \delta_{ki} D - 4 x^k x^i}{D^2} \right) \left( \frac{2 \delta_{kj} D - 4 x^k x^j}{D^2} \right) + \frac{16 x^i x^j}{D^4}.$$

    Expanding the summation yields:

    $$g_{ij} = \frac{1}{D^4} \left( 4 \delta_{ij} D^2 - 16 x^i x^j D + 16 x^i x^j (|x|^2 + 1) \right).$$

    Since $D = 1 + |x|^2$, the cross terms cancel: $-16 x^i x^j D + 16 x^i x^j (|x|^2 + 1) = -16 x^i x^j (1 + |x|^2) + 16 x^i x^j (1 + |x|^2) = 0$, leaving:

    $$g_{ij} = \frac{4 \delta_{ij} D^2}{D^4} = \frac{4 \delta_{ij}}{(1 + |x|^2)^2}.$$

Problems based on Thursday 1/22 lecture:

9. Show that $|g|_g \equiv \sqrt{n}$, where $n=\dim(M)$.

    In local coordinates, for a tensor $F$ of type $(k,l)$ with components $F^{i_1 \dots i_k}_{j_1 \dots j_l}$, the squared norm is:

   $`|F|_p^2 = g_{i_1 a_1} \cdots g_{i_k a_k} g^{j_1 b_1} \cdots g^{j_l b_l} F^{i_1 \dots i_k}_{j_1 \dots j_l} F^{a_1 \dots a_k}_{b_1 \dots b_l}`$

    For the metric $g$ itself, a $(0,2)$-tensor, this becomes $|g|^2 = g^{ij}g_{ij} = g^{ij}g_{ji} = \mathrm{tr}(g^{-1}g) = \mathrm{tr}(I) = n$, where $n = \dim(M)$. Thus, $|g|_p = \sqrt{n}$ at every point $p$.


10. Show that $\mathrm{div}(u X)=u \mathrm{div} X+\langle\nabla u, X\rangle_g$.
    On an oriented Riemannian manifold $(M, g)$, the divergence of a vector field $X$ satisfies

    $`(\mathrm{div} X) \mathrm{vol}_g = d(*X^\flat),`$

    where $*$ is the Hodge star operator associated to the metric $g$ and volume form $\mathrm{vol}_g$, and $X^\flat$ is the 1-form metrically dual to $X$ via the flat musical isomorphism.

    For a smooth scalar function $u$ and vector field $X$, the 1-form dual to $uX$ is $(uX)^\flat = u X^\flat$, since the flat isomorphism is linear over $C^\infty(M)$. The Hodge star is also $C^\infty(M)$-linear, so

    $*(uX)^\flat = *(u X^\flat) = u * X^\flat.$

    Thus,

    $\mathrm{div}(uX) \mathrm{vol}_g = d(*(uX)^\flat) = d(u * X^\flat).$

    Applying the Leibniz rule for the exterior derivative to the product of the 0-form $u$ and the $(n-1)$-form $* X^\flat$,

    $d(u * X^\flat) = du \wedge * X^\flat + u \, d(* X^\flat) = du \wedge * X^\flat + u (\mathrm{div} X) \mathrm{vol}_g.$

    The remaining term $du \wedge * X^\flat$ is an $n$-form. This term equals $\langle du, X^\flat \rangle_g \mathrm{vol}_g$ because $*X^\flat = i_X \mathrm{vol}_g$.

    To see this equality, both $*X^\flat$ and $i_X \mathrm{vol}_g$ are $(n-1)$-forms satisfying the same relation when wedged with an arbitrary 1-form $\omega^\flat$. By the defining property of the Hodge star,

    $\omega^\flat \wedge * X^\flat = \langle \omega^\flat, X^\flat \rangle_g \mathrm{vol}_g.$

    For the interior product, since $\omega^\flat \wedge \mathrm{vol}_g = 0$ (an $(n+1)$-form on an $n$-dimensional manifold), the Leibniz rule for the interior product gives

    $i_X (\omega^\flat \wedge \mathrm{vol}_g) = (i_X \omega^\flat) \wedge \mathrm{vol}_g + (-1)^1 \omega^\flat \wedge (i_X \mathrm{vol}_g).$

    Since $\omega^\flat \wedge \mathrm{vol}_g$ is an $(n+1)$-form on an $n$-dimensional manifold, it must be zero.

    The left side is zero, so

    $0 = (i_X \omega^\flat) \mathrm{vol}_g - \omega^\flat \wedge (i_X \mathrm{vol}_g),$

    hence

    $\omega^\flat \wedge (i_X \mathrm{vol}_g) = (i_X \omega^\flat) \mathrm{vol}_g.$

    But $i_X \omega^\flat = \omega^\flat(X) = \langle \omega^\flat, X^\flat \rangle_g$, so

    $\omega^\flat \wedge (i_X \mathrm{vol}_g) = \langle \omega^\flat, X^\flat \rangle_g \mathrm{vol}_g.$

    Since this holds for arbitrary 1-forms $\omega^\flat$, it follows that $*X^\flat = i_X \mathrm{vol}_g$. Therefore,

    $du \wedge * X^\flat = du \wedge (i_X \mathrm{vol}_g) = (i_X du) \mathrm{vol}_g = du(X) \mathrm{vol}_g = \langle du, X^\flat \rangle_g \mathrm{vol}_g.$

    By definition, $\langle du, X^\flat \rangle_g = du(X)$. The gradient is defined such that $du(X) = X u = \langle \nabla u, X \rangle_g$. Combining these gives:
    
    $\langle du, X^\flat \rangle_g = \langle \nabla u, X \rangle_g.$

    Substituting back yields

    $\mathrm{div}(uX) \mathrm{vol}_g = \langle \nabla u, X \rangle_g \mathrm{vol}_g + u (\mathrm{div} X) \mathrm{vol}_g.$

    Dividing by the nowhere-vanishing volume form $\mathrm{vol}_g$ gives the product rule

    $\mathrm{div}(uX) = u \mathrm{div} X + \langle \nabla u, X \rangle_g.$
